SimProof.v
@@ -118,27 +118,18 @@ Proof with automation.
       (L_0:=L_stack_str)
       (H_stack:=sh_empty)...
   - unfold S.c_update,S.c_eqb. rewrite eqb_refl...
-  - apply_fresh lc_bind.  as y. apply_fresh_base_simple bind_closed gather_vars. ltac_no_arg.
-    apply_fresh BC as y.
-
-    z : var
-  u : trm
-  H : term u
-  L : fset var
-  t1 : trm
-  H0 : forall x : var, x \notin L -> term (t1 ^ x)
-  H1 : forall x : var, x \notin L -> term ([z ~> u] t1 ^ x)
-  ============================
-  term (trm_abs ([z ~> u] t1))
-Qed.
+  - Admitted. (*apply_fresh lc_bind.
+ as y. apply_fresh_base_simple bind_closed gather_vars. ltac_no_arg.*)
+(* TLC skipped *)
 
 Theorem cond2 : forall M1 M2 i,
   LS_rel M1 M2 -> final_L M1 i -> final_S M2 i.
 Proof with automation.
   intros. destruct M1 as [[[[LC LH] LK] LE] Lt], M2 as [[SC SH] SR].
   inversion H0... inversion H... inversion H10...
-  simpl. rewrite H13. inversion H8... apply nth_middle.
+  simpl. rewrite H13. inversion H9... apply nth_middle.
 Qed.
+
 Definition stk_app f stk :=
   match stk with
   | stack lst => stack (f lst)
@@ -167,10 +158,17 @@ Theorem cond3 : forall LC SC H1 K1 E1 t1 R2 H2 H1' K1' E1' t1',
 Proof with automation.
   intros. inversion H... inversion H12...
   inversion H0;automation;
-  remember (map run_cst_trans E1 ++ s_out) as cur_stk_val;
+  remember (List.map run_cst_trans E1 ++ s_out) as cur_stk_val;
   remember (cloc Clab (List.length lst)) as l;
   remember ((L_out,stack cur_stk_val)::H_stack) as cur_stkh.
   (* 14 stepping rules, prove the multi and rel for each *)
+  3:
+    { (* x = newref <v1,...,vn> *)
+    destruct L as [L_str].
+    exists (cur_stkh,SH_cont,SH_tup
+      
+    
+  }
   - (* x = v1 + v2 *) exists
       ((L_out,stack ((int_w (i1+i2)) :: cur_stk_val))
         :: H_stack,SH_cont,SH_tup),
@@ -328,24 +326,6 @@ Proof with automation.
         rewrite <- AssocIns,app_assoc_reverse...
       * rewrite app_length. rewrite PeanoNat.Nat.add_comm...
 
-Inductive LS_rel :
-  (L.code * L.heap * L.eval_context * L.local_env * L.term)
-  -> (S.program * S.heap * reg_file) -> Prop :=
-  rel_LS : forall len lst SIlst
-    LC LH LK LE Lt SC o1 o2 o3 o4 o5 o6
-    (SH_stack:stack_heap) (SH_cont:stack_heap)
-    (SH_tup:tuple_heap)
-    (Slsp:heap_location) Clab,
-    LS_rel_ins (LE,Lt) (ins_seq SIlst) ->
-    LS_rel_context (LK,LE) (SH_stack,Slsp) ->
-    LS_rel_heap LH (SH_cont,SH_tup) -> LS_rel_code LC SC ->
-    SC Clab = ins_seq (lst ++ SIlst) -> List.length lst = len ->
-    LS_rel (LC, LH, LK, LE, Lt)
-      (SC, (SH_stack,SH_cont,SH_tup),
-        [(ip,loc_w (cloc Clab len));(sp,loc_w Slsp);(nat_reg 1,o1);
-        (nat_reg 2,o2);(nat_reg 3,o3);(nat_reg 4,o4);
-        (nat_reg 5,o5);(nat_reg 6,o6)]).
-
 (*other things
 0. changes in lexi heaps e.g. assignment
 1. handler related stuff
@@ -353,15 +333,7 @@ Inductive LS_rel :
 3. relating hdl-led-ctx*)
 
 Qed.
-(*
-0. redefine salt's opsem s.t. register files only have finite registrers
-1. prove a theorem that translated code only uses finite reg
-  - first prove that translated code only contains instructions
-  for registers 1 to 6
-  - inductively prove based on possible translated instructions
-  
 
-*)
 
 (*
 All changes made
